PREFIX : <https://olis.dev/GraphRoles/>
PREFIX cs: <https://olis.dev/GraphRoles>
PREFIX owl: <http://www.w3.org/2002/07/owl#>
PREFIX rdfs: <http://www.w3.org/2000/01/rdf-schema#>
PREFIX schema: <https://schema.org/>
PREFIX skos: <http://www.w3.org/2004/02/skos/core#>
PREFIX xsd: <http://www.w3.org/2001/XMLSchema#>


:Added
    a skos:Concept ;
    rdfs:isDefinedBy cs: ;
    skos:definition "The subject Real Graph is to be added to another Named Graph" ;
    skos:inScheme cs: ;
    skos:prefLabel "Added" ;
    skos:topConceptOf cs: ;
.

:Inferred
    a skos:Concept ;
    rdfs:isDefinedBy cs: ;
    skos:definition "The subject Real Graph is inferred from another Named Graph" ;
    skos:inScheme cs: ;
    skos:prefLabel "Inferred" ;
    skos:topConceptOf cs: ;
.

:Original
    a skos:Concept ;
    rdfs:isDefinedBy cs: ;
    skos:definition "The subject Real Graph is asserted without relation to another Named Graph" ;
    skos:inScheme cs: ;
    skos:prefLabel "Original" ;
    skos:topConceptOf cs: ;
.

:Removed
    a skos:Concept ;
    rdfs:isDefinedBy cs: ;
    skos:definition "The subject Real Graph is removed from another Named Graph" ;
    skos:inScheme cs: ;
    skos:prefLabel "Removed" ;
    skos:topConceptOf cs: ;
.

:Rules
    a skos:Concept ;
    rdfs:isDefinedBy cs: ;
    skos:definition "The subject Real Graph contains rules to be executed on another graph" ;
    skos:inScheme cs: ;
    skos:prefLabel "Rules" ;
    skos:topConceptOf cs: ;
.

<https://kurrawong.ai>
    a schema:Organization ;
    schema:name "KurrawongAI" ;
    schema:url "https://kurrawong.ai"^^xsd:anyURI ;
.

:1.0.0
    rdfs:label "1.0.0" ;
.

cs:
    a skos:ConceptScheme ;
    owl:versionIRI :1.0.0 ;
    owl:versionInfo "1.0.0: First public version" ;
    skos:definition "The roles that Named Graphs can play within an Olis context"@en ;
    skos:hasTopConcept
        :Added ,
        :Inferred ,
        :Original ,
        :Removed
        :Rules ;
    skos:historyNote """2025-12: Create in 2025 for Kurra tool operations

2026-01: Added Rules concept""" ;
    skos:prefLabel "Olis Graph Roles Vocabulary" ;
    schema:creator <https://kurrawong.ai> ;
    schema:dateCreated "2025-12-23"^^xsd:date ;
    schema:dateModified "2026-01-16"^^xsd:date ;
    schema:publisher <https://kurrawong.ai> ;
.