PREFIX : <https://linked.data.gov.au/def/cn/>
PREFIX ont: <https://linked.data.gov.au/def/cn>
PREFIX owl: <http://www.w3.org/2002/07/owl#>
PREFIX rdf: <http://www.w3.org/1999/02/22-rdf-syntax-ns#>
PREFIX rdfs: <http://www.w3.org/2000/01/rdf-schema#>
PREFIX schema: <https://schema.org/>
PREFIX skos: <http://www.w3.org/2004/02/skos/core#>
PREFIX xsd: <http://www.w3.org/2001/XMLSchema#>

rdf:value
    a owl:ObjectProperty ;
    rdfs:isDefinedBy rdf: ;
    rdfs:range rdfs:Resource ;
    skos:example "See the example for CompoundLiteral" ;
    skos:scopeNote "Use this property to indicate the value of a CompoundName, whether it's a literal or a complex object" ;
    schema:description "Idiomatic property used for structured values" ;
    schema:name "value" ;
.

rdfs:Literal
    a owl:Class ;
    rdfs:isDefinedBy rdfs: ;
    skos:example "See the literals values of '72' and 'Yundah' in the CompoundName example" ;
    skos:scopeNote "This class is used to represent the range value of the property :asLiteral. It is not expected to be used directly but instead specialised types of Literal are expected" ;
    schema:description "The class of literal values, eg. textual strings and integer" ;
    schema:name "Literal" ;
.

:CompoundName
    a owl:Class ;
    rdfs:isDefinedBy ont: ;
    skos:example """# An example Compound Name that is an Address,
# constructed in the manner of Australian street addresses
# and typically rendered for letter sending as:
#
# 72 Yundah Street
# Shorncliffe, QLD, 4017
# Australia
#
PREFIX : <https://linked.data.gov.au/def/cn/>
PREFIX ex: <http://example.com/>
PREFIX rdf: <http://www.w3.org/1999/02/22-rdf-syntax-ns#>
PREFIX rdfs: <http://www.w3.org/2000/01/rdf-schema#>
PREFIX schema: <https://schema.org/>

ex:72-yundah
    a :CompoundName ;
    rdfs:member [
        schema:additionalType ex:streetNumber ;
        rdf:value 72 ;
    ] ,
    [
        schema:additionalType ex:streetName ;
        rdf:value "Yundah" ;
    ] ,
    [
        schema:additionalType ex:streetType ;
        rdf:value ex:Street ;
    ] ,
    [
        schema:additionalType ex:locality ;
        rdf:value ex:Shorncliffe ;
    ] ,
    [
        schema:additionalType ex:state ;
        rdf:value ex:Queensland ;
    ] ,
    [
        schema:additionalType ex:postCode ;
        rdf:value 4017 ;
    ] ,
    [
        a :CompoundName ;
        schema:additionalType ex:country ;
        rdf:value ex:aus ;
        schema:name "Australia" ;
    ] ;
.

# An example Compound Name that is a Geographical Name,
# for an island off the coast of Brisbane, Australia
# that may be rendered as either Moreton Island or perhaps
# Moreton Is.
#
ex:moreton
    a :CompoundName ;
    rdfs:member [
        schema:additionalType ex:geographicalName ;
        rdf:value "Moreton" ;
    ] ,
    [
        a :CompoundName ;
        schema:additionalType ex:geographicalName ;
        rdf:value ex:Island ;
        schema:name "Island" ;
    ] ;
.""" ;
    schema:description "A Compound Name is a literal value, or objects that can be interpreted as literal values, that describe or name a Feature"@en ;
    schema:name "Compound Name"@en ;
.

:isNameFor
    a owl:ObjectProperty ;
    rdfs:isDefinedBy ont: ;
    owl:inverseOf schema:name ;
    skos:example """# Moreton Island is the Compound Name
# for a spatial object off the coast of Brisbane, Australia
#
PREFIX : <https://linked.data.gov.au/def/cn/>
PREFIX ex: <http://example.com/>
PREFIX geo: <http://www.opengis.net/ont/geosparql#>

ex:moreton
    a :CompoundName ;
    :isNameFor ex:feature-x ;
.

ex:feature-x
    a geo:Feature ;
    schema:name ex:moreton ;
.""" ;
    schema:description "Links a name to the thing it is used for" ;
    schema:name "is name for" ;
.

schema:additionalType
    a owl:ObjectProperty ;
    rdfs:domain rdfs:Resource ;
    rdfs:isDefinedBy schema: ;
    rdfs:range rdfs:Resource ;
    skos:example "See the example for CompoundLiteral" ;
    skos:scopeNote "Use this property to indicate the specialised type of a part of a CompoundName" ;
    schema:description "An additional type for the item, typically used for adding more specific types from external vocabularies" ;
    schema:name "additional type" ;
.

schema:hasPart
    a owl:ObjectProperty ;
    rdfs:isDefinedBy schema: ;
    skos:example "See the example for CompoundName" ;
    skos:scopeNote "Use this property to indicate the individual parts of a Compound Name" ;
    schema:description "Indicates a Resource that is part of this item" ;
    schema:name "member" ;
.

schema:name
    a owl:DatatypeProperty ;
    rdfs:isDefinedBy schema: ;
    skos:example "See example for isNameFor" ;
    skos:usageNote "In this model, name is used to indicate both a literal form of a resource`s name or a CompoundName object" ;
    schema:description "The name of the item" ;
    schema:name "name" ;
.

:0.0.1 schema:name "0.0.1" .

ont:
    a owl:Ontology ;
    owl:versionIRI :0.0.2 ;
    owl:versionInfo "0.0.2" ;
    skos:historyNote """This ontology was made for the Queensland Department of Resources, Spatial Information unit in 2023 to assist with future Address, Place Names, Roads & Cadastre systems design however it is intended to provide background modelling for all ANZ jurisdictions' foundational spatial data.

This model has been made with the FSDF Supermodel in mind (https://linked.data.gov.au/def/fsdf-supermodel) so that is compatible with that, and the Locaiton Index (Loc-I) projects' modelling and goals."""@en ;
    schema:codeRepository "https://github.com/AGLDWG/compound-naming-model/"^^xsd:anyURI ;
    schema:copyrightHolder <https://orcid.org/0000-0002-8742-7730> ;
    schema:copyrightNotice "(c) Nicholas J. Car, 2023" ;
    schema:creator <https://orcid.org/0000-0002-8742-7730> ;
    schema:dateCreated "2023-04-26"^^xsd:date ;
    schema:dateIssued "2023-04-26"^^xsd:date ;
    schema:dateModified "2022-04-26"^^xsd:date ;
    schema:description "This model allows for the representation of compound names that can be assigned to be assigned to features"@en ;
    schema:license
        <https://rdflicense.linkeddata.es/rdflicense/cc-by4.0> ,
        "https://creativecommons.org/licenses/by/4.0/"^^xsd:anyURI ;
    schema:name "Compound Naming Model"@en ;
    schema:publisher <https://linked.data.gov.au/org/agldwg> ;
.

rdfs:Resource
    a owl:Class ;
    rdfs:isDefinedBy rdfs: ;
    skos:example "See the non-literal values for rdf:value in the CompoundName example" ;
    skos:scopeNote "This class is used to represent both the things to which CompoundNames can be assigned and also the range value of the property rdf:value. It is not expected to be used directly but instead specialised types of Resource are expected" ;
    schema:description "The class resource, everything" ;
    schema:name "Resource" ;
.
